split up files and more cases+lemmas

Linear/Basic.lean
@@ -1,70 +1,9 @@
 import Mathlib.Data.Multiset.Basic
+import Mathlib.Tactic.Abel
+import Linear.Defs
+import Linear.Lemmas
+import Linear.Tactic
 
-inductive Ty : Type where
-  | Plus : Ty → Ty → Ty
-  | Tensor : Ty → Ty → Ty
-  | Lolly : Ty → Ty → Ty
-  | With : Ty → Ty → Ty
-  | One
-
-infixr:69 " ⊸ " => Ty.Lolly
-infixl:70 " ⊕ " => Ty.Plus
-infixl:71 " ⊗ " => Ty.Tensor
-infixl:72 " & " => Ty.With
-
-@[reducible]
-def Cx : Type := Multiset Ty
-
-inductive Typed : Cx → Ty → Prop where
-  | One_R 
-    : Typed ∅ Ty.One
-
-  | One_L {Δ : Cx} {C : Ty} 
-    : Typed Δ C → Typed (Ty.One ::ₘ Δ) C
-
-  | Tensor_L {Δ : Cx} {A B C : Ty}
-    : Typed (A ::ₘ B ::ₘ Δ) C → Typed (A ⊗ B ::ₘ Δ) C
-
-  | Tensor_R {A B : Ty} (Δ₁ Δ₂ : Cx) 
-    : Typed Δ₁ A → Typed Δ₂ B → Typed (Δ₁ + Δ₂) (A ⊗ B)
-
-  | Plus_L {Δ : Cx} {A B C : Ty}
-    : Typed (A ::ₘ Δ) C → Typed (B ::ₘ Δ) C → Typed ((A ⊕ B) ::ₘ Δ) C
-
-  | Plus_R1 {Δ : Cx} {A B : Ty}
-    : Typed Δ A → Typed Δ (A ⊕ B)
-
-  | Plus_R2 {Δ : Cx} {A B : Ty}
-    : Typed Δ B → Typed Δ (A ⊕ B)
-
-  | Lolly_L (Δ₁ Δ₂ : Cx) {A B C : Ty}
-    : Typed Δ₁ A → Typed (B ::ₘ Δ₂) C → Typed (A ⊸ B ::ₘ (Δ₁ + Δ₂)) C
-
-  | Lolly_R {Δ : Cx} {A B : Ty}
-    : Typed (A ::ₘ Δ) B → Typed Δ (A ⊸ B)
-
-  | With_L1 {Δ : Cx} {A B C : Ty}
-    : Typed (A ::ₘ Δ) C → Typed (A & B ::ₘ Δ) C
-
-  | With_L2 {Δ : Cx} {A B C : Ty}
-    : Typed (B ::ₘ Δ) C → Typed (A & B ::ₘ Δ) C
-
-  | With_R {Δ : Cx} {A B : Ty}
-    : Typed Δ A → Typed Δ B → Typed Δ (A & B)
-
-
-infix:50 " ⊢ " => Typed
-
-syntax "apply_triv" : tactic
-macro_rules
-  | `(tactic|apply_triv) =>
-  `(tactic|
-    repeat' (
-      first | apply Typed.One_R | apply Typed.One_L | 
-        apply Typed.Tensor_L | apply Typed.Lolly_R |
-        apply Typed.With_R | apply Typed.Tensor_R
-      try simp only [Multiset.cons_zero]
-        ) ) 
 
 -- syntax "apply_triv1" : tactic
 -- macro_rules
@@ -112,30 +51,10 @@ theorem typed_id : {a} ⊢ a := by
     apply Typed.Lolly_L {a} {} <;> assumption
 
 
-lemma mem_of_cons {Δ1 Δ2 : Cx} {a1 a2 : Ty} 
-  : a1 ≠ a2 → a1 ::ₘ Δ1 = a2 ::ₘ Δ2 → a2 ∈ Δ1 := by
-  intros hne hce
-  have : a2 ∈ a2 ::ₘ Δ2 := Multiset.mem_cons_self a2 Δ2
-  rw [←hce] at this
-  apply Multiset.mem_cons.mp at this
-  cases this with
-  | inr => assumption
-  | inl h => 
-    rw [Eq.comm] at h
-    contradiction
 
-lemma cons_mem_of_add {Δ Δ1 Δ2: Cx} {a : Ty} (h : a ::ₘ Δ = Δ1 + Δ2)
-  : ∃ Δ', Δ1 = a ::ₘ Δ' ∨ Δ2 = a ::ₘ Δ' := by 
-    have : a ∈ Δ1 ∨ a ∈ Δ2 := by
-      rw [←Multiset.mem_add, ←h]
-      exact Multiset.mem_cons_self _ _
-    cases this <;> {
-      rename_i hm
-      obtain ⟨Δ', hΔ'⟩ := Multiset.exists_cons_of_mem hm;
-      exists Δ'
-      subst hΔ'
-      simp
-    }
+
+
+
 
 
 -- syntax "cut_r_l" tactic : tactic
@@ -144,8 +63,67 @@ lemma cons_mem_of_add {Δ Δ1 Δ2: Cx} {a : Ty} (h : a ::ₘ Δ = Δ1 + Δ2)
 --   `(tactic|
 --     ) 
 
+/-
+The individual proofs typically follow at least one of the following forms, in
+order:
+
+1. h is of the form `a ::ₘ Δ₁ = b ::ₘ Δ₂` where `a ≠ b`
+  - we want to introduce Δ as a common context using `exists_common_of_eq`
 
 
+-/
+
+lemma cut_elim_one_r (h2 : Ty.One ::ₘ Δ' ⊢ B) : ∅ + Δ' ⊢ B := by
+  generalize h : Ty.One ::ₘ Δ' = Δ'' at h2
+  induction h2 generalizing Δ'
+  case One_R => 
+    absurd h
+    exact Multiset.cons_ne_zero
+  case One_L a b c d => 
+    simp at *
+    rw [h]
+    exact c
+  case Tensor_L Δ2 c d b2 hb2 IH3 =>
+    simp at *
+    have : c ⊗ d ∈ Δ' := mem_of_cons (by simp) h
+    obtain ⟨Δ'2, hΔ'2⟩ := Multiset.exists_cons_of_mem this
+    rw [hΔ'2]
+    apply Typed.Tensor_L
+    apply IH3
+    rw [Multiset.cons_swap]; simp
+    rw [Multiset.cons_swap]; simp
+    rw [hΔ'2] at h
+    rw [Multiset.cons_swap] at h; simp at h
+    assumption
+  case Tensor_R c d Δt1 Δt2 hc hd IH IH' =>
+    simp at *
+    obtain ⟨Δ, hΔ⟩ := cons_mem_of_add h
+    cases hΔ <;> {
+      subst_vars
+      simp at h IH IH'
+      subst h
+      constructor <;> assumption
+    }
+  case Plus_L IH IH' =>
+    obtain ⟨_, hΔ'2⟩ := Multiset.exists_cons_of_mem (mem_of_cons (by simp) h)
+    subst hΔ'2; repeat (rw [Multiset.cons_swap] at h; simp at h)
+    simp
+    subst h
+    rw [Multiset.cons_swap] at IH IH'
+    simp at IH IH'
+    constructor <;> assumption
+  case Plus_R1 IH =>
+    apply Typed.Plus_R1
+    subst h
+    simp at IH
+    simp [IH]
+  case Plus_R2 IH =>
+    apply Typed.Plus_R2
+    subst h
+    simp at IH
+    simp [IH]
+    
+  repeat1 sorry
 
 theorem cut_elim {Δ Δ' : Cx} {A B : Ty} (h1 : Δ ⊢ A) (h2 : A ::ₘ Δ' ⊢ B)
   : Δ + Δ' ⊢ B := by
@@ -154,31 +132,7 @@ theorem cut_elim {Δ Δ' : Cx} {A B : Ty} (h1 : Δ ⊢ A) (h2 : A ::ₘ Δ' ⊢ 
     rw [Multiset.cons_add]
     apply Typed.One_L
     exact IH h2
-  case One_R => 
-    generalize h : Ty.One ::ₘ Δ' = Δ'' at h2
-    induction h2 generalizing Δ'
-    case One_R => 
-      absurd h
-      exact Multiset.cons_ne_zero
-    case One_L a b c d => 
-      simp at *
-      rw [h]
-      exact c
-    case Tensor_L Δ2 c d b2 hb2 IH3 =>
-      simp at *
-      have : c ⊗ d ∈ Δ' := mem_of_cons (by simp) h
-      obtain ⟨Δ'2, hΔ'2⟩ := Multiset.exists_cons_of_mem this
-      rw [hΔ'2]
-      apply Typed.Tensor_L
-      apply IH3
-      rw [Multiset.cons_swap]; simp
-      rw [Multiset.cons_swap]; simp
-      rw [hΔ'2] at h
-      rw [Multiset.cons_swap] at h; simp at h
-      assumption
-
-      
-    repeat sorry
+  case One_R => exact cut_elim_one_r h2
   case With_R Δ1 a b ha hb IH1 IH2 =>
     generalize h : (a & b) ::ₘ Δ' = Δ'' at h2
     induction h2 generalizing Δ'
@@ -220,42 +174,34 @@ theorem cut_elim {Δ Δ' : Cx} {A B : Ty} (h1 : Δ ⊢ A) (h2 : A ::ₘ Δ' ⊢ 
       assumption
     case One_R => simp at h
     case One_L IH =>
+      -- canonical basic case
       obtain ⟨_, hΔ'2⟩ := Multiset.exists_cons_of_mem (mem_of_cons (by simp) h)
-      rw [hΔ'2]
-      rw [hΔ'2] at h; repeat (rw [Multiset.cons_swap] at h; simp at h)
+      subst hΔ'2; repeat (rw [Multiset.cons_swap] at h; simp at h)
       rw [add_comm, Multiset.cons_add]
       apply Typed.One_L
 
       rw [add_comm]
-      apply IH <;> try assumption
+      apply IH <;> assumption
     case Lolly_L Δl1 Δl2 la lb lc hla hlc IH IH' => 
       obtain ⟨Δ'2, hΔ'2⟩ := Multiset.exists_cons_of_mem (mem_of_cons _ h)
       subst_vars
       repeat (simp [Multiset.cons_swap] at h)
       rw [add_comm, Multiset.cons_add]
-      have : (a & b) ∈ Δl1 ∨ (a & b) ∈ Δl2 := by
-        rw [←Multiset.mem_add, ←h]
-        exact Multiset.mem_cons_self _ _
-      cases this with
+      obtain ⟨Δl1', hΔl1'⟩ := cons_mem_of_add h
+      cases hΔl1' with
       | inl hi =>
-        apply Multiset.exists_cons_of_mem at hi
-        obtain ⟨Δl1', hΔl1'⟩ := hi
         subst_eqs
         simp at h IH
         subst h
         rw [add_right_comm]
         rw [add_comm] at IH
         apply Typed.Lolly_L <;> assumption
-      
       | inr hi => 
-        apply Multiset.exists_cons_of_mem at hi
-        obtain ⟨Δl1', hΔl1'⟩ := hi
         subst_eqs
         simp at h
         subst h
         rw [add_right_comm, add_assoc]
         apply Typed.Lolly_L <;> try assumption
-
         rw [add_comm, ←Multiset.cons_add, add_comm]
         apply IH'
         simp [Multiset.cons_swap]
@@ -303,19 +249,204 @@ theorem cut_elim {Δ Δ' : Cx} {A B : Ty} (h1 : Δ ⊢ A) (h2 : A ::ₘ Δ' ⊢ 
         subst_eqs
         apply IH2
         assumption
-    case Tensor_R c d Δc Δd hc hd IH' IH =>
+    case Tensor_R c d Δc Δd hc hd IH IH' =>
+      obtain ⟨Δ, hΔ⟩ := cons_mem_of_add h
+      cases hΔ with
+      | inl hc =>
+        subst hc
+        simp at h IH
+        subst h
+        rw [←add_assoc]
+        apply Typed.Tensor_R <;> assumption
+      | inr hc => 
+        subst hc
+        simp at h IH IH'
+        subst h
+        rw [←add_comm, add_right_comm, add_assoc]
+        apply Typed.Tensor_R <;> assumption
+    case Plus_R1 Δ c d hc IH => 
+      apply Typed.Plus_R1
+      exact IH h
+    case Plus_R2 Δ c d hc IH => 
+      apply Typed.Plus_R2
+      exact IH h
+    case Lolly_R Δ c d hc IH =>
+      apply Typed.Lolly_R
+      rw [add_comm, ←Multiset.cons_add, add_comm]
+      apply IH
+      simp [Multiset.cons_swap]
+      assumption
+    case With_R Δ c d hc hd IH IH' => 
+      apply Typed.With_R
+      exact IH h
+      exact IH' h
+  case Tensor_R a b Δt1 Δt2 ha hb IH1_outer IH2_outer =>
+    generalize h : (a ⊗ b) ::ₘ Δ' = Δ'' at h2
+    generalize ht : Δt1 + Δt2 = Δt at *
+    induction h2 generalizing Δ'
+    case Lolly_L Δl1 Δl2 la lb lc hla hlc IH IH' => 
+      let ⟨Δ, ⟨hΔ1, hΔ2⟩⟩ := exists_common_of_eq (by simp) h
+      subst hΔ1
+      obtain ⟨Δ, ⟨hΔ'⟩⟩ := cons_mem_of_add (Eq.symm hΔ2)
+      case inl =>
+        subst hΔ'
+        simp at hΔ2; subst hΔ2
+        clear h
+        simp at *
+        -- what I want to be able to do is automatically put the goal in a form
+        -- that can be unified with IH, but I haven't quite figured that out.
+        -- My best guess is a tactic that looks at the de-generalized IH and
+        -- the Typed constructor to re-apply, but that seems clearly wrong
+        rw [←add_assoc]
+        apply Typed.Lolly_L <;> assumption
+      case inr hΔ' => -- I have no clue why it isn't bound here automatically
+        subst hΔ'
+        simp at hΔ2; subst hΔ2
+        clear h
+        rw [Multiset.cons_swap] at IH'
+        simp at *
+        rw [add_left_comm]
+        apply Typed.Lolly_L <;> assumption
+    case One_R => absurd h; simp
+    case One_L IH =>
+      let ⟨Δ, ⟨hΔ1, hΔ2⟩⟩ := exists_common_of_eq (by simp) h
+      subst hΔ1
+      subst hΔ2
+      simp at *
+      apply Typed.One_L <;> assumption
+    case Tensor_L Δ c d e he IH =>
+      -- every case that's the inverse of the outer needs the by_cases
+      by_cases heq : a ⊗ b ≠ c ⊗ d
+      case pos =>
+        let ⟨Δ, ⟨hΔ1, hΔ2⟩⟩ := exists_common_of_eq heq h
+        substs hΔ1 hΔ2
+        clear h
+        rw [cons_rot] at IH
+        simp at IH
+        rw [add_comm, Multiset.cons_add, add_comm]
+        apply Typed.Tensor_L <;> assumption
+      case neg =>
+        clear IH -- impossible to satisfy
+        simp at heq
+        obtain ⟨x, x⟩ := heq; subst_vars
+        simp at h; subst h
+        rw [add_assoc, add_left_comm]
+        apply_assumption
+        rw [add_comm, ←Multiset.cons_add, add_comm]
+        apply_assumption
+        assumption
+    case Tensor_R IH1 IH2 =>
+      obtain ⟨Δ, ⟨hΔ⟩⟩ := cons_mem_of_add h
+      case inl =>
+        subst hΔ
+        simp at h
+        subst h
+        simp at IH1
+        rw [←add_assoc]
+        constructor <;> solve_by_elim
+      case inr hΔ =>
+        subst hΔ
+        simp at h
+        subst h
+        rw [add_left_comm]
+        constructor <;> solve_by_elim
+    case Plus_L IH1 IH2 =>
+      let ⟨Δ, ⟨hΔ1, hΔ2⟩⟩ := exists_common_of_eq (by simp) h
+      substs hΔ1 hΔ2
+      clear h -- trivial
+      rw [Multiset.cons_swap] at IH1 IH2; simp at IH1 IH2
+      simp
+      constructor <;> assumption
+    case Plus_R1 IH1 IH2 => solve_by_elim [Typed.Plus_R1]
+    case Plus_R2 IH1 IH2 => solve_by_elim [Typed.Plus_R2]
+    case With_L1 IH =>
+      let ⟨Δ, ⟨hΔ1, hΔ2⟩⟩ := exists_common_of_eq (by simp) h
+      substs hΔ1 hΔ2
+      clear h
+      rw [Multiset.cons_swap] at IH; simp at IH
+      simp
+      -- can omit this apply since it's the first ctor
+      -- apply Typed.With_L2
+      solve_by_elim
+    case With_L2 IH =>
+      let ⟨Δ, ⟨hΔ1, hΔ2⟩⟩ := exists_common_of_eq (by simp) h
+      substs hΔ1 hΔ2
+      clear h
+      rw [Multiset.cons_swap] at IH; simp at IH
+      simp
+      apply Typed.With_L2
+      solve_by_elim
+    case With_R IH1 IH2 =>
+      subst h
+      simp at IH1 IH2
+      solve_by_elim
+    case Lolly_R IH =>
+      subst h
+      rw [Multiset.cons_swap] at IH; simp at IH
+      solve_by_elim
+  case Tensor_L Δ a b c IH1_outer IH2_outer =>
+    simp at IH2_outer
+    generalize h : c ::ₘ Δ' = Δ'' at h2
+    induction h2 generalizing Δ'
+    case One_R => absurd h; simp
+    case One_L IH => 
+      by_cases hne: c ≠ Ty.One
+      let ⟨Δ, ⟨hΔ1, hΔ2⟩⟩ := exists_common_of_eq hne h
+      case pos =>
+        substs hΔ1 hΔ2
+        clear h
+        simp at IH
+        simp; solve_by_elim
+      case neg =>
+        clear IH
+        simp at hne
+        subst hne
+        simp at h
+        subst h
+        rw [Multiset.cons_add]
+        constructor
+        solve_by_elim
+    case Tensor_L d e f g h IH =>
+      by_cases hne: c ≠ e ⊗ f
+      case pos =>
+        let ⟨Δ, ⟨hΔ1, hΔ2⟩⟩ := exists_common_of_eq hne h
+        subst_vars
+        clear h
+        -- rw [cons_rot] at IH; simp at IH
+        simp_cx at IH
 
-      sorry
 
 
 
-
-
-
-
-      
-
-
-      
+        -- simp; constructor
+        -- rw [cons_rot]
+        -- assumption
+      case neg =>
+        simp at hne
+        subst hne
+        simp at h
+        subst h
+        simp; constructor
+        solve_by_elim
+    case Tensor_R IH1 IH2 =>
+      obtain ⟨Δ, ⟨hΔ⟩⟩ := cons_mem_of_add h
+      case inl =>
+        subst hΔ
+        simp at h
+        subst h
+        simp at IH1 IH2
+        rw [←add_assoc]
+        -- while solve_by_elim or constructor frequently works, it's more
+        -- reliable to apply the specific case
+        apply Typed.Tensor_R
+        · simp; assumption
+        · solve_by_elim
+      case inr hΔ =>
+        subst hΔ
+        simp at h
+        subst h
+        simp at IH1 IH2
+        rw [←add_assoc]
+        apply Typed.Tensor_R
 
 
