Linear/Defs.lean
@@ -1,0 +1,56 @@
+import Mathlib.Data.Multiset.Basic
+
+inductive Ty : Type where
+  | Plus : Ty → Ty → Ty
+  | Tensor : Ty → Ty → Ty
+  | Lolly : Ty → Ty → Ty
+  | With : Ty → Ty → Ty
+  | One
+
+infixr:69 " ⊸ " => Ty.Lolly
+infixl:70 " ⊕ " => Ty.Plus
+infixl:71 " ⊗ " => Ty.Tensor
+infixl:72 " & " => Ty.With
+
+@[reducible]
+def Cx : Type := Multiset Ty
+
+inductive Typed : Cx → Ty → Prop where
+  | One_R 
+    : Typed ∅ Ty.One
+
+  | One_L {Δ : Cx} {C : Ty} 
+    : Typed Δ C → Typed (Ty.One ::ₘ Δ) C
+
+  | Tensor_L {Δ : Cx} {A B C : Ty}
+    : Typed (A ::ₘ B ::ₘ Δ) C → Typed (A ⊗ B ::ₘ Δ) C
+
+  | Tensor_R {A B : Ty} (Δ₁ Δ₂ : Cx) 
+    : Typed Δ₁ A → Typed Δ₂ B → Typed (Δ₁ + Δ₂) (A ⊗ B)
+
+  | Plus_L {Δ : Cx} {A B C : Ty}
+    : Typed (A ::ₘ Δ) C → Typed (B ::ₘ Δ) C → Typed ((A ⊕ B) ::ₘ Δ) C
+
+  | Plus_R1 {Δ : Cx} {A B : Ty}
+    : Typed Δ A → Typed Δ (A ⊕ B)
+
+  | Plus_R2 {Δ : Cx} {A B : Ty}
+    : Typed Δ B → Typed Δ (A ⊕ B)
+
+  | Lolly_L (Δ₁ Δ₂ : Cx) {A B C : Ty}
+    : Typed Δ₁ A → Typed (B ::ₘ Δ₂) C → Typed (A ⊸ B ::ₘ (Δ₁ + Δ₂)) C
+
+  | Lolly_R {Δ : Cx} {A B : Ty}
+    : Typed (A ::ₘ Δ) B → Typed Δ (A ⊸ B)
+
+  | With_L1 {Δ : Cx} {A B C : Ty}
+    : Typed (A ::ₘ Δ) C → Typed (A & B ::ₘ Δ) C
+
+  | With_L2 {Δ : Cx} {A B C : Ty}
+    : Typed (B ::ₘ Δ) C → Typed (A & B ::ₘ Δ) C
+
+  | With_R {Δ : Cx} {A B : Ty}
+    : Typed Δ A → Typed Δ B → Typed Δ (A & B)
+
+
+infix:50 " ⊢ " => Typed
