Linear/Lemmas.lean
@@ -1,0 +1,44 @@
+import Linear.Defs
+
+lemma mem_of_cons {Δ1 Δ2 : Cx} {a1 a2 : Ty} 
+  : a1 ≠ a2 → a1 ::ₘ Δ1 = a2 ::ₘ Δ2 → a2 ∈ Δ1 := by
+  intros hne hce
+  have : a2 ∈ a2 ::ₘ Δ2 := Multiset.mem_cons_self a2 Δ2
+  rw [←hce] at this
+  apply Multiset.mem_cons.mp at this
+  cases this with
+  | inr => assumption
+  | inl h => 
+    rw [Eq.comm] at h
+    contradiction
+
+lemma cons_mem_of_add {Δ Δ1 Δ2: Cx} {a : Ty} (h : a ::ₘ Δ = Δ1 + Δ2)
+  : ∃ Δ', Δ1 = a ::ₘ Δ' ∨ Δ2 = a ::ₘ Δ' := by 
+    have : a ∈ Δ1 ∨ a ∈ Δ2 := by
+      rw [←Multiset.mem_add, ←h]
+      exact Multiset.mem_cons_self _ _
+    cases this <;> {
+      rename_i hm
+      obtain ⟨Δ', hΔ'⟩ := Multiset.exists_cons_of_mem hm;
+      exists Δ'
+      subst hΔ'
+      simp
+    }
+
+lemma exists_common_of_eq {a b : Ty} 
+  (hne : a ≠ b) (h : a ::ₘ Δ₁ = b ::ₘ Δ₂)
+  : ∃ Δ, Δ₁ = b ::ₘ Δ ∧ Δ₂ = a ::ₘ Δ := by 
+  obtain ⟨Δ, hΔ⟩ := Multiset.exists_cons_of_mem $ mem_of_cons hne h
+  exists Δ
+  subst hΔ
+  rw [Multiset.cons_swap, Eq.comm] at h
+  simp at h
+  simp [h]
+
+
+
+lemma rot4' {a b c d : Cx} : a + b + c + d = d + a + b + c := by ac_rfl
+lemma rot4 {a b c d : Cx} : a + b + c + d = b + c + d + a := by ac_rfl
+
+lemma cons_rot {Δ : Cx} : a ::ₘ b ::ₘ c ::ₘ Δ = c ::ₘ a ::ₘ b ::ₘ Δ := by
+  simp_rw [Multiset.cons_swap]
