Linear/Tactic.lean
@@ -1,0 +1,26 @@
+import Lean
+import Lean.Parser.Syntax
+import Lean.Parser.Tactic
+import Linear.Defs
+import Linear.Lemmas
+
+syntax "apply_triv" : tactic
+macro_rules
+  | `(tactic|apply_triv) =>
+  `(tactic|
+    repeat' (
+      first | apply Typed.One_R | apply Typed.One_L | 
+        apply Typed.Tensor_L | apply Typed.Lolly_R |
+        apply Typed.With_R | apply Typed.Tensor_R
+      try simp only [Multiset.cons_zero]
+        ) ) 
+
+syntax "simp_cx " (Lean.Parser.Tactic.location)? : tactic
+macro_rules
+  | `(tactic|simp_cx $l?) =>
+  `(tactic| 
+    simp [] $l?; -- put it in the simp normal form
+    (iterate 2 try (rewrite [cons_rot] $l?; simp [] $l?));
+    (try (rw [Multiset.cons_swap] $l?; simp [] $l?));
+    try simp [] $l?; -- put it back in normal form
+  ) 
